src/Equivalence/Basics.v
@@ -1,5 +1,10 @@
+From CoreErlang.Equivalence Require Export Tactics.
 From CoreErlang Require Export Basics.
 Require Export stdpp.list.
+
+(**
+* foldl_ext
+*)
 
 (**
 NOTES:  Maybe place this in CoreErlang/Basics
@@ -8,11 +13,16 @@ NOTES:  Maybe place this in CoreErlang/Basics
 
 
 Lemma foldl_ext :
-  forall (A B : Type) (f1 f2 : A -> B -> A) (x1 x2 : A) (l1 l2 : list B),
-    (forall (a : A) (b : B), f1 a b = f2 a b) ->
-    l1 = l2 ->
-    x1 = x2 ->
-    fold_left f1 l1 x1 = fold_left f2 l2 x2.
+  forall
+    (A B : Type)
+    (f1 f2 : A -> B -> A)
+    (x1 x2 : A)
+    (l1 l2 : list B),
+      (forall (a : A) (b : B), f1 a b = f2 a b)
+  ->  l1 = l2
+  ->  x1 = x2
+  ->  fold_left f1 l1 x1
+  =   fold_left f2 l2 x2.
 Proof.
   intros A B f1 f2 x1 x2 l1 l2 Hf Hl Hx.
   rewrite Hl.
