src/Equivalence/BigStepToFrameStack/Induction.v
@@ -1,0 +1,192 @@
+From CoreErlang.BigStep Require Export Syntax Induction.
+
+Import ListNotations.
+
+(**
+* Value
+* Expression
+*)
+
+(**
+NOTES:  Maybe place this in BigStep/Induction
+*)
+
+
+
+
+
+
+
+
+
+Section Value.
+
+
+
+  Variables
+    (P : Value -> Prop).
+
+
+
+  Hypotheses
+    (HNil : P VNil)
+
+    (HLit :
+      forall l,
+        P (VLit l))
+
+    (HCons :
+      forall hd tl,
+          P hd
+      ->  P tl
+      ->  P (VCons hd tl))
+
+    (HClos :
+      forall ref ext id params body funid,
+          Forall (fun x => P (snd x)) ref
+      ->  P (VClos ref ext id params body funid))
+
+    (HTuple :
+      forall l,
+          Forall P l
+      ->  P (VTuple l))
+
+    (HMap :
+      forall l,
+          Forall (fun x => P (fst x) /\ P (snd x)) l
+      ->  P (VMap l)).
+
+
+
+  Theorem value_ind :
+    forall v, P v.
+  Proof.
+    induction v using Value_ind2 with
+      (Q := Forall P)
+      (R := Forall (fun x => P (fst x) /\ P (snd x)))
+      (W := Forall (fun x => P (snd x))); intuition.
+  Defined.
+
+
+
+End Value.
+
+
+
+
+
+
+Section Expression.
+
+
+
+  Variables
+    (P : Expression -> Prop).
+
+
+
+  Hypotheses
+    (HValues :
+      forall el,
+          Forall P el
+      ->  P (EValues el))
+
+    (HNil : P ENil)
+
+    (HLit :
+      forall l,
+          P (ELit l))
+
+    (HVar :
+      forall v,
+          P (EVar v))
+
+    (HFunId :
+      forall f,
+        P (EFunId f))
+
+    (HFun :
+      forall vl e,
+          P e
+      ->  P (EFun vl e))
+
+    (HCons :
+      forall hd tl,
+          P hd
+      ->  P tl
+      ->  P (ECons hd tl))
+
+    (HTuple :
+      forall l,
+          Forall P l
+      ->  P (ETuple l))
+
+    (HCall :
+      forall m f l,
+          P m
+      ->  P f
+      ->  Forall P l
+      ->  P (ECall m f l))
+
+    (HPrimOp :
+      forall f l,
+          Forall P l
+      ->  P (EPrimOp f l))
+
+    (HApp :
+      forall exp l,
+          P exp
+      ->  Forall P l
+      ->  P (EApp exp l))
+
+    (HCase :
+      forall e l,
+          P e
+      ->  Forall (fun x => P (snd (fst x)) /\ P (snd x)) l
+      ->  P (ECase e l))
+
+    (HLet :
+      forall l e1 e2,
+          P e1
+      ->  P e2
+      ->  P (ELet l e1 e2))
+
+    (HSeq :
+      forall e1 e2,
+          P e1
+      ->  P e2
+      ->  P (ESeq e1 e2))
+
+    (HLetRec :
+      forall l e,
+          P e
+      ->  Forall (fun x => P (snd (snd x))) l
+      ->  P (ELetRec l e))
+
+    (HMap :
+      forall l,
+          Forall (fun x => P (fst x) /\ P (snd x)) l
+      ->  P (EMap l))
+
+    (HTry :
+      forall e1 vl1 e2 vl2 e3,
+          P e1
+      ->  P e2
+      ->  P e3
+      ->  P (ETry e1 vl1 e2 vl2 e3)).
+
+
+
+  Theorem exp_ind :
+    forall e, P e.
+  Proof.
+    induction e using Expression_ind2 with
+      (Q := Forall P)
+      (R := Forall (fun x => P (fst x) /\ P (snd x)))
+      (W := Forall (fun x => P (snd (fst x)) /\ P (snd x)))
+      (Z := Forall (fun x => P (snd (snd x)))); intuition.
+  Defined.
+
+
+
+End Expression.
