src/Equivalence/BigStepToFrameStack/Simple/MeasureLemmas.v
@@ -1,275 +1,527 @@
-From CoreErlang.Equivalence.BigStepToFrameStack.Simple Require Export Substitute.
+From CoreErlang.Equivalence.BigStepToFrameStack.Simple Require Export SubstituteLemmas.
 From CoreErlang.Equivalence.BigStepToFrameStack Require Export Measure.
+
+From CoreErlang.Equivalence.BigStepToFrameStack Require Import Induction.
 
 Import BigStep.
 
 (**
-* meausre_reduction [Admitted]
-* meausre_reduction_list [Admitted]
-* meausre_reduction_map [Admitted]
+* Value
+  - measure_val_reduction
+  - measure_val_reduction_list
+  - measure_val_reduction_map
+  - measure_val_reduction_min
+* EnvExpression
+  - measure_env_exp_reduction
+  - measure_env_exp_reduction_min
 *)
 
 
 
+Section Value.
 
-(*
-Theorem subst_env_empty :
-  forall n e,
-    subst_env n [] e = e.
-Proof.
-  intros.
-  destruct n.
-  { by cbn. }
-  induction e using derived_Expression_ind.
-  * 
-Admitted.
-*)
 
-Theorem measure_reduction_val :
-  forall v n1 n2,
-    measure_val v <= n1
-  ->
-    measure_val v <= n2
-  ->
-    bval_to_bexp (subst_env n1) v
-  =
-    bval_to_bexp (subst_env n2) v.
-Proof.
-  intros v n1 n2 Hn1 Hn2.
-  induction v using derived_Value_ind.
-  * by cbn.
-  * by cbn.
-  * (* Cons *)
-    remember
-      (BigStep.Syntax.VCons v1 v2)
-      as vcons
-      eqn:Heq_vcons.
-    assert (measure_val v1 ≤ measure_val vcons) as Hv1.
-    rewrite Heq_vcons; slia.
-    assert (measure_val v2 ≤ measure_val vcons) as Hv2.
-    rewrite Heq_vcons; slia.
-    assert (measure_val v1 ≤ n1) as Hv1n1.
-    {
-      apply Nat.le_trans with (m := measure_val vcons).
-      - exact Hv1.
-      - exact Hn1.
-    }
-    assert (measure_val v1 ≤ n2) as Hv1n2.
-    {
-      apply Nat.le_trans with (m := measure_val vcons).
-      - exact Hv1.
-      - exact Hn2.
-    }
-    assert (measure_val v2 ≤ n1) as Hv2n1.
-    {
-      apply Nat.le_trans with (m := measure_val vcons).
-      - exact Hv2.
-      - exact Hn1.
-    }
-    assert (measure_val v2 ≤ n2) as Hv2n2.
-    {
-      apply Nat.le_trans with (m := measure_val vcons).
-      - exact Hv2.
-      - exact Hn2.
-    }
-    clear Hv1 Hv2 Hn1 Hn2.
-    specialize (IHv1 Hv1n1 Hv1n2).
-    specialize (IHv2 Hv2n1 Hv2n2).
-    inv Heq_vcons.
-    clear H Hv1n1 Hv1n2 Hv2n1 Hv2n2.
-    cbn.
-    rewrite IHv1.
-    rewrite IHv2.
-    reflexivity.
-  * (* Clos *)
-    induction ref as [| x env IHenv].
-    - cbn.
-      admit.
-    - admit.
-  * (* Tuple *)
-    induction l as [| v vl IHvl].
-    - by cbn.
-    - inv H.
-      rename H2 into Hv.
-      rename H3 into HForall.
+
+  Theorem measure_val_reduction :
+    forall v n1 n2,
+      measure_val v <= n1
+    ->
+      measure_val v <= n2
+    ->
+      bval_to_bexp (subst_env n1) v
+    =
+      bval_to_bexp (subst_env n2) v.
+  Proof.
+    intros v n1 n2 Hn1 Hn2.
+    induction v using derived_Value_ind.
+    * by cbn.
+    * by cbn.
+    * (* Cons *)
       remember
-        (BigStep.Syntax.VTuple vl)
-        as vtuple_vl
-        eqn:Heq_vtuple_vl.
-      remember
-        (BigStep.Syntax.VTuple (v :: vl))
-        as vtuple_vvl
-        eqn:Heq_vtuple_vvl.
-      assert (measure_val vtuple_vl ≤ measure_val vtuple_vvl) as Hvl.
-      {
-        rewrite Heq_vtuple_vl.
-        rewrite Heq_vtuple_vvl.
-        simpl.
-        unfold measure_list.
-        simpl.
-        slia.
-      }
-      assert (measure_val v ≤ n1) as Hvn1.
-      {
-        apply Nat.le_trans with (m := measure_val vtuple_vvl).
-        - inv Heq_vtuple_vvl. cbn. lia.
-        - exact Hn1.
-      }
-      assert (measure_val vtuple_vl ≤ n1) as Hvln1.
-      {
-        apply Nat.le_trans with (m := measure_val vtuple_vvl).
-        - exact Hvl.
-        - exact Hn1.
-      }
-      assert (measure_val v ≤ n2) as Hvn2.
-      {
-        apply Nat.le_trans with (m := measure_val vtuple_vvl).
-        - inv Heq_vtuple_vvl. cbn. lia.
-        - exact Hn2.
-      }
-      assert (measure_val vtuple_vl ≤ n2) as Hvln2.
-      {
-        apply Nat.le_trans with (m := measure_val vtuple_vvl).
-        - exact Hvl.
-        - exact Hn2.
-      }
-      clear Hn1 Hn2.
-      specialize (Hv Hvn1 Hvn2).
-      specialize (IHvl HForall Hvln1 Hvln2).
-      inv Heq_vtuple_vl.
-      clear H Hvn1 Hvln1 Hvn2 Hvln2 Hvl HForall.
-      simpl in *.
-      injection IHvl as Hmap_vl.
-      rewrite Hmap_vl.
-      rewrite Hv.
-      reflexivity.
-  * (* Map *)
-    induction l as [| (v1, v2) vl IHvl].
-    - by cbn.
-    - inv H.
-      rename H2 into Hv.
-      rename H3 into HForall.
-      simpl in Hv.
-      destruct Hv as [Hv1 Hv2].
-      remember
-        (BigStep.Syntax.VMap vl)
-        as vmap_vl
-        eqn:Heq_vmap_vl.
-      remember
-        (BigStep.Syntax.VMap ((v1, v2) :: vl))
-        as vmap_vvl
-        eqn:Heq_vmap_vvl.
-      assert (measure_val vmap_vl ≤ measure_val vmap_vvl) as Hvl.
-      {
-        rewrite Heq_vmap_vl.
-        rewrite Heq_vmap_vvl.
-        simpl.
-        unfold measure_list.
-        unfold measure_map.
-        slia.
-      }
+        (BigStep.Syntax.VCons v1 v2)
+        as vcons
+        eqn:Heq_vcons.
+      assert (measure_val v1 ≤ measure_val vcons) as Hv1.
+      rewrite Heq_vcons; slia.
+      assert (measure_val v2 ≤ measure_val vcons) as Hv2.
+      rewrite Heq_vcons; slia.
       assert (measure_val v1 ≤ n1) as Hv1n1.
       {
-        apply Nat.le_trans with (m := measure_val vmap_vvl).
-        - inv Heq_vmap_vvl. cbn. lia.
-        - exact Hn1.
-      }
-      assert (measure_val v2 ≤ n1) as Hv2n1.
-      {
-        apply Nat.le_trans with (m := measure_val vmap_vvl).
-        - inv Heq_vmap_vvl. cbn. lia.
-        - exact Hn1.
-      }
-      assert (measure_val vmap_vl ≤ n1) as Hvln1.
-      {
-        apply Nat.le_trans with (m := measure_val vmap_vvl).
-        - exact Hvl.
+        apply Nat.le_trans with (m := measure_val vcons).
+        - exact Hv1.
         - exact Hn1.
       }
       assert (measure_val v1 ≤ n2) as Hv1n2.
       {
-        apply Nat.le_trans with (m := measure_val vmap_vvl).
-        - inv Heq_vmap_vvl. cbn. lia.
+        apply Nat.le_trans with (m := measure_val vcons).
+        - exact Hv1.
         - exact Hn2.
+      }
+      assert (measure_val v2 ≤ n1) as Hv2n1.
+      {
+        apply Nat.le_trans with (m := measure_val vcons).
+        - exact Hv2.
+        - exact Hn1.
       }
       assert (measure_val v2 ≤ n2) as Hv2n2.
       {
-        apply Nat.le_trans with (m := measure_val vmap_vvl).
-        - inv Heq_vmap_vvl. cbn. lia.
+        apply Nat.le_trans with (m := measure_val vcons).
+        - exact Hv2.
         - exact Hn2.
       }
-      assert (measure_val vmap_vl ≤ n2) as Hvln2.
+      clear Hv1 Hv2 Hn1 Hn2.
+      specialize (IHv1 Hv1n1 Hv1n2).
+      specialize (IHv2 Hv2n1 Hv2n2).
+      inv Heq_vcons.
+      clear H Hv1n1 Hv1n2 Hv2n1 Hv2n2.
+      cbn.
+      rewrite IHv1.
+      rewrite IHv2.
+      reflexivity.
+    * (* Clos *)
+      rename H into HForall.
+      induction ref as [| x env IHenv].
+      - cbn.
+        destruct ext; destruct funid.
+        1-2, 4: rewrite rem_vars_empty; by do 2 rewrite subst_env_empty.
+        rewrite rem_nfifes_empty.
+        f_equal.
+        unfold bval_to_bexp_ext.
+        apply map_ext.
+        intros [fid [vl e]].
+        rewrite rem_vars_empty.
+        do 2 rewrite subst_env_empty.
+        reflexivity.
+      - inv HForall.
+        rename H1 into Hx.
+        rename H2 into HForall.
+        specialize (IHenv HForall).
+        clear HForall.
+        remember
+          (VClos env ext id params body funid)
+          as v_env
+          eqn:Heq_v_env.
+        remember
+          (VClos (x :: env) ext id params body funid)
+          as v_xenv
+          eqn:Heq_v_xenv.
+        assert (measure_val v_env ≤ measure_val v_xenv) as Henv.
+        {
+          rewrite Heq_v_env.
+          rewrite Heq_v_xenv.
+          simpl.
+          unfold measure_env.
+          slia.
+        }
+        assert (measure_val x.2 ≤ n1) as Hxn1.
+        {
+          apply Nat.le_trans with (m := measure_val v_xenv).
+          - rewrite Heq_v_xenv. destruct x. simpl. unfold measure_env. slia.
+          - exact Hn1.
+        }
+        assert (measure_val v_env ≤ n1) as Henvn1.
+        {
+          apply Nat.le_trans with (m := measure_val v_xenv).
+          - exact Henv.
+          - exact Hn1.
+        }
+        assert (measure_val x.2 ≤ n2) as Hxn2.
+        {
+          apply Nat.le_trans with (m := measure_val v_xenv).
+          - rewrite Heq_v_xenv. destruct x. simpl. unfold measure_env. slia.
+          - exact Hn2.
+        }
+        assert (measure_val v_env ≤ n2) as Henvn2.
+        {
+          apply Nat.le_trans with (m := measure_val v_xenv).
+          - exact Henv.
+          - exact Hn2.
+        }
+        specialize (Hx Hxn1 Hxn2).
+        specialize (IHenv Henvn1 Henvn2).
+        clear Hxn1 Hxn2 Henvn1 Henvn2 Henv.
+        inv Heq_v_env.
+        clear H Hn2 Hn1.
+        simpl in *.
+        destruct ext; destruct funid.
+        + f_equal.
+          inv IHenv.
+          rename H0 into Henv.
+          destruct x.
+          simpl in *.
+          admit.
+        + admit.
+        + admit.
+        + admit.
+    * (* Tuple *)
+      induction l as [| v vl IHvl].
+      - by cbn.
+      - inv H.
+        rename H2 into Hv.
+        rename H3 into HForall.
+        remember
+          (BigStep.Syntax.VTuple vl)
+          as vtuple_vl
+          eqn:Heq_vtuple_vl.
+        remember
+          (BigStep.Syntax.VTuple (v :: vl))
+          as vtuple_vvl
+          eqn:Heq_vtuple_vvl.
+        assert (measure_val vtuple_vl ≤ measure_val vtuple_vvl) as Hvl.
+        {
+          rewrite Heq_vtuple_vl.
+          rewrite Heq_vtuple_vvl.
+          simpl.
+          unfold measure_list.
+          simpl.
+          slia.
+        }
+        assert (measure_val v ≤ n1) as Hvn1.
+        {
+          apply Nat.le_trans with (m := measure_val vtuple_vvl).
+          - inv Heq_vtuple_vvl. cbn. lia.
+          - exact Hn1.
+        }
+        assert (measure_val vtuple_vl ≤ n1) as Hvln1.
+        {
+          apply Nat.le_trans with (m := measure_val vtuple_vvl).
+          - exact Hvl.
+          - exact Hn1.
+        }
+        assert (measure_val v ≤ n2) as Hvn2.
+        {
+          apply Nat.le_trans with (m := measure_val vtuple_vvl).
+          - inv Heq_vtuple_vvl. cbn. lia.
+          - exact Hn2.
+        }
+        assert (measure_val vtuple_vl ≤ n2) as Hvln2.
+        {
+          apply Nat.le_trans with (m := measure_val vtuple_vvl).
+          - exact Hvl.
+          - exact Hn2.
+        }
+        clear Hn1 Hn2.
+        specialize (Hv Hvn1 Hvn2).
+        specialize (IHvl HForall Hvln1 Hvln2).
+        inv Heq_vtuple_vl.
+        clear H Hvn1 Hvln1 Hvn2 Hvln2 Hvl HForall.
+        simpl in *.
+        injection IHvl as Hmap_vl.
+        rewrite Hmap_vl.
+        rewrite Hv.
+        reflexivity.
+    * (* Map *)
+      induction l as [| (v1, v2) vl IHvl].
+      - by cbn.
+      - inv H.
+        rename H2 into Hv.
+        rename H3 into HForall.
+        simpl in Hv.
+        destruct Hv as [Hv1 Hv2].
+        remember
+          (BigStep.Syntax.VMap vl)
+          as vmap_vl
+          eqn:Heq_vmap_vl.
+        remember
+          (BigStep.Syntax.VMap ((v1, v2) :: vl))
+          as vmap_vvl
+          eqn:Heq_vmap_vvl.
+        assert (measure_val vmap_vl ≤ measure_val vmap_vvl) as Hvl.
+        {
+          rewrite Heq_vmap_vl.
+          rewrite Heq_vmap_vvl.
+          simpl.
+          unfold measure_list.
+          unfold measure_map.
+          slia.
+        }
+        assert (measure_val v1 ≤ n1) as Hv1n1.
+        {
+          apply Nat.le_trans with (m := measure_val vmap_vvl).
+          - inv Heq_vmap_vvl. cbn. lia.
+          - exact Hn1.
+        }
+        assert (measure_val v2 ≤ n1) as Hv2n1.
+        {
+          apply Nat.le_trans with (m := measure_val vmap_vvl).
+          - inv Heq_vmap_vvl. cbn. lia.
+          - exact Hn1.
+        }
+        assert (measure_val vmap_vl ≤ n1) as Hvln1.
+        {
+          apply Nat.le_trans with (m := measure_val vmap_vvl).
+          - exact Hvl.
+          - exact Hn1.
+        }
+        assert (measure_val v1 ≤ n2) as Hv1n2.
+        {
+          apply Nat.le_trans with (m := measure_val vmap_vvl).
+          - inv Heq_vmap_vvl. cbn. lia.
+          - exact Hn2.
+        }
+        assert (measure_val v2 ≤ n2) as Hv2n2.
+        {
+          apply Nat.le_trans with (m := measure_val vmap_vvl).
+          - inv Heq_vmap_vvl. cbn. lia.
+          - exact Hn2.
+        }
+        assert (measure_val vmap_vl ≤ n2) as Hvln2.
+        {
+          apply Nat.le_trans with (m := measure_val vmap_vvl).
+          - exact Hvl.
+          - exact Hn2.
+        }
+        clear Hn1 Hn2.
+        specialize (Hv1 Hv1n1 Hv1n2).
+        specialize (Hv2 Hv2n1 Hv2n2).
+        specialize (IHvl HForall Hvln1 Hvln2).
+        inv Heq_vmap_vl.
+        clear H Hv1n1 Hv2n1 Hvln1 Hv1n2 Hv2n2 Hvln2 Hvl HForall.
+        simpl in *.
+        injection IHvl as Hvl.
+        rewrite Hv1.
+        rewrite Hv2.
+        rewrite Hvl.
+        reflexivity.
+  Admitted.
+
+
+
+  Theorem measure_val_reduction_list :
+    forall vl v1 v2,
+      list_sum (map measure_val vl) <= measure_val v1
+    ->
+      list_sum (map measure_val vl) <= measure_val v2
+    ->
+      map (bval_to_bexp (subst_env (measure_val v1))) vl
+    =
+      map (bval_to_bexp (subst_env (measure_val v2))) vl.
+  Proof.
+    intros vl v1 v2 Hv1 Hv2.
+    induction vl.
+    * by cbn.
+    * rename a into v.
+      assert (measure_val v
+        <= list_sum (map measure_val (v :: vl))) as Hv.
+      slia.
+      assert (list_sum (map measure_val vl)
+        <= list_sum (map measure_val (v :: vl))) as Hvl.
+      slia.
+      assert (measure_val v <= measure_val v1) as Hvv1.
       {
-        apply Nat.le_trans with (m := measure_val vmap_vvl).
-        - exact Hvl.
-        - exact Hn2.
+        apply Nat.le_trans with (m := list_sum (map measure_val (v :: vl))).
+          - exact Hv.
+          - exact Hv1.
       }
-      clear Hn1 Hn2.
-      specialize (Hv1 Hv1n1 Hv1n2).
-      specialize (Hv2 Hv2n1 Hv2n2).
-      specialize (IHvl HForall Hvln1 Hvln2).
-      inv Heq_vmap_vl.
-      clear H Hv1n1 Hv2n1 Hvln1 Hv1n2 Hv2n2 Hvln2 Hvl HForall.
-      simpl in *.
-      injection IHvl as Hvl.
-      rewrite Hv1.
-      rewrite Hv2.
+      assert (list_sum (map measure_val vl) <= measure_val v1) as Hvlv1.
+      {
+        apply Nat.le_trans with (m := list_sum (map measure_val (v :: vl))).
+          - exact Hvl.
+          - exact Hv1.
+      }
+      assert (measure_val v <= measure_val v2) as Hvv2.
+      {
+        apply Nat.le_trans with (m := list_sum (map measure_val (v :: vl))).
+          - exact Hv.
+          - exact Hv2.
+      }
+      assert (list_sum (map measure_val vl) <= measure_val v2) as Hvlv2.
+      {
+        apply Nat.le_trans with (m := list_sum (map measure_val (v :: vl))).
+          - exact Hvl.
+          - exact Hv2.
+      }
+      clear Hv Hvl Hv1 Hv2.
+      specialize (IHvl Hvlv1 Hvlv2).
+      pose proof measure_val_reduction
+        v (measure_val v1) (measure_val v2) Hvv1 Hvv2 as Hv.
+      clear Hvv1 Hvlv1 Hvv2 Hvlv2.
+      cbn.
+      rewrite IHvl.
+      rewrite Hv.
+      reflexivity.
+  Qed.
+
+
+
+  Theorem measure_val_reduction_map :
+    forall vl v1 v2,
+      list_sum (map (fun '(x, y) => (measure_val x) + (measure_val y)) vl)
+        <= measure_val v1
+    ->
+      list_sum (map (fun '(x, y) => (measure_val x) + (measure_val y)) vl)
+        <= measure_val v2
+    ->
+      map
+        (prod_map
+          (bval_to_bexp (subst_env (measure_val v1)))
+          (bval_to_bexp (subst_env (measure_val v1))))
+        vl
+    =
+      map
+        (prod_map
+          (bval_to_bexp (subst_env (measure_val v2)))
+          (bval_to_bexp (subst_env (measure_val v2))))
+        vl.
+  Proof.
+    intros vl v1 v2 Hvvl_v1 Hvvl_v2.
+    induction vl.
+    * by cbn.
+    * (* + rename/remember *)
+      rename a into v.
+      remember
+        (measure_val v1)
+        as measure_v1
+        eqn: Heq_v1.
+      remember
+        (measure_val v2)
+        as measure_v2
+        eqn: Heq_v2.
+      remember
+        (measure_val v.1)
+        as measure_vx
+        eqn: Heq_vx.
+      remember
+        (measure_val v.2)
+        as measure_vy
+        eqn: Heq_vy.
+      remember
+        (measure_val v.1 + measure_val v.2)
+        as measure_v
+        eqn: Heq_v.
+      remember
+        (list_sum (map (λ '(x, y), measure_val x + measure_val y) vl))
+        as measure_vl
+        eqn: Heq_vl.
+      remember
+        (list_sum (map (λ '(x, y), measure_val x + measure_val y) (v :: vl)))
+        as measure_vvl
+        eqn: Heq_vvl.
+      (* + assert triv *)
+      assert (measure_vx <= measure_v) as Hvx_v.
+      slia.
+      assert (measure_vy <= measure_v) as Hvy_v.
+      slia.
+      assert (measure_v <= measure_vvl) as Hv_vvl.
+      rewrite Heq_v; rewrite Heq_vvl; destruct v; slia.
+      assert (measure_vl <= measure_vvl) as Hvl_vvl.
+      rewrite Heq_vl; rewrite Heq_vvl; slia.
+      (* + assert trans *)
+      assert (measure_vx <= measure_v1) as Hvx_v1.
+      {
+        apply Nat.le_trans with (m := measure_vvl).
+        - apply Nat.le_trans with (m := measure_v).
+          + exact Hvx_v.
+          + exact Hv_vvl.
+        - exact Hvvl_v1.
+      }
+      assert (measure_vy <= measure_v1) as Hvy_v1.
+      {
+        apply Nat.le_trans with (m := measure_vvl).
+        - apply Nat.le_trans with (m := measure_v).
+          + exact Hvy_v.
+          + exact Hv_vvl.
+        - exact Hvvl_v1.
+      }
+      assert (measure_vl <= measure_v1) as Hvl_v1.
+      {
+        apply Nat.le_trans with (m := measure_vvl).
+        - exact Hvl_vvl.
+        - exact Hvvl_v1.
+      }
+      assert (measure_vx <= measure_v2) as Hvx_v2.
+      {
+        apply Nat.le_trans with (m := measure_vvl).
+        - apply Nat.le_trans with (m := measure_v).
+          + exact Hvx_v.
+          + exact Hv_vvl.
+        - exact Hvvl_v2.
+      }
+      assert (measure_vy <= measure_v2) as Hvy_v2.
+      {
+        apply Nat.le_trans with (m := measure_vvl).
+        - apply Nat.le_trans with (m := measure_v).
+          + exact Hvy_v.
+          + exact Hv_vvl.
+        - exact Hvvl_v2.
+      }
+      assert (measure_vl <= measure_v2) as Hvl_v2.
+      {
+        apply Nat.le_trans with (m := measure_vvl).
+        - exact Hvl_vvl.
+        - exact Hvvl_v2.
+      }
+      rewrite Heq_vx in *.
+      rewrite Heq_vy in *.
+      clear Heq_vx Heq_vy Hvx_v Hvy_v Hv_vvl Hvl_vvl Hvvl_v1 Hvvl_v2.
+      (* + specialize/pose proof *)
+      pose proof measure_val_reduction
+        v.1 measure_v1 measure_v2 Hvx_v1 Hvx_v2 as Hvx.
+      pose proof measure_val_reduction
+        v.2 measure_v1 measure_v2 Hvy_v1 Hvy_v2 as Hvy.
+        specialize (IHvl Hvl_v1 Hvl_v2) as Hvl.
+      clear - Hvx Hvy Hvl.
+      (* rewrite *)
+      destruct v as [x y].
+      cbn in *.
+      rewrite Hvx.
+      rewrite Hvy.
       rewrite Hvl.
       reflexivity.
-Admitted.
+  Qed.
+
+
+
+  Theorem measure_val_reduction_min :
+    forall v n,
+        measure_val v <= n
+    ->  bval_to_bexp (subst_env n) v
+    =   bval_to_bexp (subst_env (measure_val v)) v.
+  Proof.
+    intros v n Hn.
+    assert (measure_val v <= measure_val v) as Hv.
+    lia.
+    by pose proof measure_val_reduction
+      v n (measure_val v) Hn Hv.
+  Qed.
+
+
+
+End Value.
 
 
 
 
 
 
-Theorem measure_reduction_val_list :
-  forall vl v1 v2,
-    list_sum (map measure_val vl) <= measure_val v1
-  ->
-    list_sum (map measure_val vl) <= measure_val v2
-  ->
-    map (bval_to_bexp (subst_env (measure_val v1))) vl
-  =
-    map (bval_to_bexp (subst_env (measure_val v2))) vl.
-Proof.
-Admitted.
+Section EnvExpression.
 
 
 
+  Theorem measure_env_exp_reduction :
+    forall env e n1 n2,
+        measure_env_exp env e <= n1
+    ->  measure_env_exp env e <= n2
+    ->  subst_env n1 env e
+    =   subst_env n2 env e.
+  Proof.
+  Admitted.
 
 
 
-Theorem measure_reduction_val_map :
-  forall ml v1 v2,
-    list_sum (map (fun '(x, y) => (measure_val x) + (measure_val y)) ml)
-      <= measure_val v1
-  ->
-    list_sum (map (fun '(x, y) => (measure_val x) + (measure_val y)) ml)
-      <= measure_val v2
-  ->
-    map
-      (prod_map
-        (bval_to_bexp (subst_env (measure_val v1)))
-        (bval_to_bexp (subst_env (measure_val v1))))
-      ml
-  =
-    map
-      (prod_map
-        (bval_to_bexp (subst_env (measure_val v2)))
-        (bval_to_bexp (subst_env (measure_val v2))))
-      ml.
-Proof.
-Admitted.
+  Theorem measure_env_exp_reduction_min :
+    forall env e n,
+        measure_env_exp env e <= n
+    ->  subst_env n env e
+    =   subst_env (measure_env_exp env e) env e.
+  Proof.
+    intros env e n Hn.
+    assert (measure_env_exp env e <= measure_env_exp env e) as Hv.
+    lia.
+    by pose proof measure_env_exp_reduction
+      env e n (measure_env_exp env e) Hn Hv.
+  Qed.
 
 
 
-
-
-
-Theorem measure_reduction_subst_env :
-  forall env e n,
-    measure_env_exp env e <= n
-    -> subst_env n env e = subst_env (measure_env_exp env e) env e.
-Proof.
-Admitted.
+End EnvExpression.
