src/Equivalence/Tactics.v
@@ -1,0 +1,25 @@
+From CoreErlang Require Export Basics.
+
+(**
+NOTES:  Maybe place this in CoreErlang/Tactics
+*)
+
+
+
+Ltac clear_refl
+  :=
+repeat match goal with
+| H : ?x = ?x |- _ => clear H
+end.
+
+Ltac refold
+  x
+  :=
+unfold x;
+fold x.
+
+Ltac invc
+  H
+  :=
+inv H;
+clear_refl.
